\part{Exercice 4}

On a $\|u\|^2 = 2$ d'où $e_1 = \frac{1}{\sqrt{2}}(1, 0, 1)$.

\begin{align*}
	v  - \left<v \mid e_1 \right>e_1 &= (1,1,1) - \frac{1}{\sqrt{2}} \times 2 \times \frac{1}{\sqrt{2}}(1,0,1) \\
	&= (0, 1, 0) \\
\end{align*}

D'où $e_2 = \frac{(0,1,0)}{\|(0,1,0)\|} = (0, 1, 0)$.

\begin{align*}
	w - \left<w \mid e_1 \right> e_1 - \left<w  \mid e_2 \right> e_2
	&= (-1, 1, 0) + \frac{1}{\sqrt{2}}\times \frac{1}{\sqrt{2}} \times (1, 0, 1) - (0,1,0) \\
	&= \left( -\frac{1}{2}, 0, \frac{1}{2} \right) \\
\end{align*}

On a $\left\|\left( -\frac{1}{2}, 0, \frac{1}{2} \right) \right\|^2 = \frac{1}{4} + \frac{1}{4} = \frac{1}{2}$ d'où \[
	e_3 = \frac{\left( -\frac{1}{2}, 0, \frac{1}{2} \right)}{\left\|\left( -\frac{1}{2}, 0, \frac{1}{2} \right)\right\|} = \left( -\frac{\sqrt{2}}{2}, 0, \frac{\sqrt{2}}{2} \right)
.\]


