\part{Exercice 1}

\begin{enumerate}
	\item On a \[
			\left|
			\begin{array}{c c c}
				0&a&b\\
				a&0&c\\ \cline{1-3}
				\multicolumn{1}{|c}{b}&c&\multicolumn{1}{c|}{0}\\\cline{1-3}
			\end{array}
			\right| = abc + abc = 2abc.
		\] 
	\item
		\begin{align*}
			\begin{vmatrix}
				a&b&c\\
				c&a&b\\
				b&c&a\\
			\end{vmatrix} &= a(a^2 - cb) - b(ca - b^2) + c(c^2 - ba)\\
			&= a^3 - abc - abc + b^3 + c^3 - abc \\
			&= a^3 -3abc + b^3 + c^3 \\
		\end{align*}
	\item{\Large \ding{96}}
	\item
		\begin{align*}
			\begin{vmatrix}
				a&a&a&a\\
				a&b&b&b\\
				a&b&c&c\\
				a&b&c&d\\
			\end{vmatrix} &=
			\begin{vmatrix}
				a&a&a&a\\
				0&b-a&b-a&b-a\\
				0&b-a&c-a&c-a\\
				0&b-a&c-a&d-a\\
			\end{vmatrix}\\
			&= 
			\begin{vmatrix}
				a&a&a&a\\
				0&b-a&b-a&b-a\\
				0&0&c-b&c-b\\
				0&0&c-b&d-c\\
			\end{vmatrix}\\
			&= 
			\begin{vmatrix}
				a&a&a&a\\
				0&b-a&b-a&b-a\\
				0&0&c-b&c-b\\
				0&0&0&d-c
			\end{vmatrix}\\
			&= a(b-a)(c-d)(d-c) \\
		\end{align*}
\end{enumerate}

