\part{Exercice 10}

On pose 
\begin{align*}
	P &= (X - x)(X - y)(X - z)\\
	&= X^3 - (x + y + z)X^2 + (xy + xz + yz)X - xyz \\
\end{align*}

On pose \[
	\begin{cases}
		\s = x + y + z\\
		p = xyz\\
		q = xy + xz + yz
	\end{cases}
\]
On sait que $\s = 0$.
\begin{align*}
	\s^2 &= (x + y + z)^2\\
	&= x^2 + y^2 + z^2 + \underbrace{2xy + 2yz + 2xz}_{2q} \\
\end{align*}

donc, \[
	\frac{x^2+y^2+z^2}{2}=-q
\]

\begin{align*}
	0 = P(x) = x^3 - \s x^2 + qx - p\\
	0 = P(y) = y^3 - \s y^2 + qy - p\\
	0 = P(z) = z^3 - \s z^2 + qz - p\\
\end{align*}

D'o√π, \[
	x^3 + y^3 + z^3 = -q\s +  3p = 3q
\] donc \[
	\frac{x^3 + y^3 + z^3}{3}=p
\]

On a aussi

\begin{align*}
	0 = x^5 + qx^3 - px^2\\
	0 = y^5 + qy^3 - py^2\\
	0 = z^5 + qz^3 - pz^2\\
\end{align*}

et donc \[
	x^5 + y^5 + z^5 = -3qp - 2qp = -5qp
\] donc \[
	\frac{x^5 + y^5 + z^5}{5} = -qp = \frac{x^2+y^2+z^2}{2} \times \frac{x^3 + y^3 + z^3}{3}
\]
