\part{Exercice 4}

On a $\|u\| = \sqrt{2}$ donc $a = \left( \frac{\sqrt{2}}{2},0,\frac{\sqrt{2}}{2} \right)$.

On pose
\begin{align*}
	b &= v - \left<v \mid a \right> a\\
	&= v - 2\frac{\sqrt{2}}{2} \left( \frac{\sqrt{2}}{2}, 0, \frac{\sqrt{2}}{2} \right)  \\
	&= (1,1,1) - (1, 0, 1) \\
	&= (0,1,0) \\
\end{align*}

On a bien $\|b\| = 1$.

On pose
\begin{align*}
	c &= w - \left<w \mid a \right>a - \left<w \mid b \right>b\\
	&= (-1, 1, 0) - 0 \times a - 1\times b \\
	&= (-1, 0, 0) \\
\end{align*}

