\part{Exercice 3}

\begin{enumerate}
	\item[a.]
		\begin{align*}
			\forall  n \in \N, u_n &= \sqrt{n\left( 1+\frac{1}{n} \right)} - \sqrt{n}\\
										&= \sqrt{n}\left(1- \frac{1}{2n} + o\left( \frac{1}{n} \right) -1  \right) \\
										&\sim -\frac{1}{2\sqrt{n}} \tendsto{n \to +\infty} 0\\
		\end{align*}
	\item[b.] $\forall n \in \N_*$ \\
		$n - (-1)^n = n\left(1 - \frac{(-1)^n}{n}\right) \sim n$ \\
		car $\left| \frac{(-1)^n}{n} \right| = \frac{1}{n} \tendsto{n \to +\infty} 0$ \\
		De mÃªme, $n + (-1)^n \sim n$ donc $u_n \sim \frac{n}{n} = 1 \tendsto{n \to +\infty} 1$ 
	\item[c.] $\forall n \in \N_*$
		\begin{align*}
			u_n &= \left( 2 + (-1)^n \right) ^{\frac{1}{n}} \\
			&= e^{\frac{1}{n}\ln\left( 2 + (-1)^n \right) } \\
			&= e^{\frac{1}{n} + O(1)} \tendsto{n \to +\infty} 1 \\
			&\text{car } \frac{1}{n}O(1) \tendsto{n \to +\infty} 0
		\end{align*}
	\item[e.] $\forall k \in \N,$
		\[
			kx - 1 < \left\lfloor kx \right\rfloor \le kx
		\] Donc $\forall n \in \N_*$,\[
			\frac{1}{n^2} \sum_{k=1}^n(kx -1) < u_n \le \frac{1}{n^2}\sum_{k=1}^n kx
		\] Donc $\forall n \in \N_*$, \[
			\underbrace{\frac{1}{n^2}\left( \frac{xn(n+1)}{2} - n \right)}_{\sim \frac{x}{2}} \le u_n \le \underbrace{\frac{x}{n^2} \times \frac{n(n+1)}{2}}_{\sim \frac{x}{2}}	
		\]
		Donc, $u_n \tendsto{n \to +\infty} \frac{x}{2}$ 
	\item[g.]
		$\forall n \in \N_*$ \\
		\[
			\sum_{k=1}^{2n+1} \frac{1}{n+1} \le \sum_{k=1}^{2n+1} \frac{1}{\sqrt{n^2+k}} \le \sum_{k=1}^{2n+1}\frac{1}{n}
		\] donc, $\forall n \in \N_*$, \[
			\underbrace{\frac{2n+1}{n+1}}_{\tendsto{n\to +\infty}2} \le u_n \le \underbrace{\frac{2n+1}{n}}_{\tendsto{n\to +\infty}2}
		\] donc $u_n \tendsto{n \to +\infty} 2$
	\item[l.] $\forall n \in \N_*, u_n = \frac{n!}{n^n}$\\
		\begin{align*}
			\forall n \ge 2, 0 \le u_n &= \frac{1 \times 2 \times  3 \times \ldots \times n}{n \times n \times n \times \ldots \times n}\\
			&= \frac{1}{n} \times \frac{2}{n} \times \ldots \times \frac{n}{n} \\
			&= \frac{1}{n}\prod_{k=2}^n \frac{k}{n} \le \frac{1}{n} \tendsto{n \to +\infty} 0 \\
		\end{align*}
\end{enumerate}









