\part{Exercice 9}

\begin{center}
	\Large Hyper classique!
\end{center}

\begin{enumerate}
	\item $f: x \mapsto \frac{1}{x}$ \\
		\begin{center}
			\begin{asy}
				import graph;
				import patterns;

				add("hatch1",hatch(2mm, heavycyan));
				add("hatch2",hatch(2mm, magenta));

				size(5cm);

				real f(real x) {return 1/x;}

				real a = 3;
				real k = 2.5;

				draw(graph(f, 1/a, a + 2));
				axes(EndArrow);

				label("\small $k$", (k,-0.25));
				label("\small $k-1$", (k-1,-0.25));
				label("\small $k+1$", (k+1,-0.25));

				draw((k,0) -- (k, f(k)), dotted);
				draw((k-1,0) -- (k-1, f(k-1)), dotted);
				draw((k+1,0) -- (k+1, f(k+1)), dotted);

				filldraw((k-1, 0) -- (k-1,f(k)) -- (k,f(k)) -- (k,0) -- cycle, pattern("hatch1"), heavycyan);
				filldraw((k+1, 0) -- (k+1,f(k)) -- (k,f(k)) -- (k,0) -- cycle, pattern("hatch2"), magenta);
			\end{asy}
		\end{center}
		\[
			\forall k > 2,
			\int_{k}^{k+1} \frac{1}{x} dx \le \frac{1}{k} \le \int_{k-1}^{k} \frac{1}{x} dx
		\]

		Or, \[
			\ln(k+1) - \ln(k) \le \frac{1}{k} \le \ln(k) - \ln(k-1)
		\] donc \[
			\forall k \ge  2,
			\ln\left( \frac{k-1}{k} \right) \le \frac{1}{k}
		\] et  \[
			\forall k \ge 1, \frac{1}{k+1}\le \ln\left( \frac{k+1}{k} \right)
		\]
	\item Soit $n \in \N_*$ \\
		\begin{align*}
			u_{n+1} - u_n &= \sum_{k=1}^{n+1} \frac{1}{k} - \ln(n+1) - \sum_{k=1}^{n}\frac{1}{k} + \ln(n)\\
			&= \frac{1}{n+1} - \ln\left( \frac{n+1}{n} \right) \le 0\\
		\end{align*}
		\begin{align*}
			v_{n+1} - v_n &= \sum_{k=1}^{n+1}\frac{1}{k}- \ln(n+2) + \sum_{k=1}^n \frac{1}{k} + \ln(n+1)\\
			&= \frac{1}{n+1} - \ln\left( \frac{n+2}{n+1} \right)  \\
		\end{align*}
		\[
			u_n - v_n = -\ln(n+1) +\ln(n) = \ln\left( \frac{n}{n+1} \right) \tendsto{n\to +\infty} 0
		\] 
	\item $(u_n)$ converge, on note $\gamma$ sa limite: \[
			u_n = \gamma + o(1)
		\] 
		donc \[
			\sum_{k=1}^n \frac{1}{k} - \ln(n) = \gamma + o(1)
		\] donc
		\begin{center}
			\fbox{$\sum_{k=1}^n \frac{1}{k} = \ln(n) + \gamma + o(1)$}
		\end{center}
	\item $S_n \sim \ln(n) \tendsto{n \to +\infty} +\infty$
	\item
		\begin{align*}
			\sum_{k=n}^{2n}\frac{1}{k} &= \sum_{k=1}^{2n}\frac{1}{k} - \sum_{k=1}^{n-1} \frac{1}{k} \\
			&= \ln(2n) + \gamma + o(1) - \ln(n-1) - \gamma + o(1)\\
			&= \ln\left( \frac{2n}{n-1}+o(1) \right) \\
			&\tendsto{n \to +\infty} \ln 2
		\end{align*}
\end{enumerate}
