\part{Exercice 8}

\begin{itemize}
	\item[\underline{\sc Analyse}] Soient $n \in \N^*$ et $f \in S_n$ tels que $g : \begin{array}{rcl}
			\left\llbracket 1,b \right\rrbracket &\longrightarrow& \left\llbracket 0,n-1 \right\rrbracket \\
			k &\longmapsto& \big|f(k) - k\big|
		\end{array}$ injective. Donc $g$ est bijective et donc \[
			\sum_{k=1}^n g(k) = \sum_{i=0}^{n-1} i = \frac{n(n-1)}{2}.
		\]

		\[
			\forall k,\; g(k) \equiv f(k)-k\mod 2
		\] donc
		\begin{align*}
			\sum_{k=1}^n g(k) &\equiv \sum_{k=1}^n \big(f(k) - k\big) \mod 2\\
			&\equiv 0\mod 2
		\end{align*}
		donc \[
			n(n-1) \equiv 0\mod 4
		\] donc $\begin{cases}
			n \equiv 0\mod 4\\
			n-1\equiv 0 \mod 4
		\end{cases}$
	\item[\underline{\sc Synth√®se}] On suppose $n\equiv 0\mod 4$ : $n = 4p$.
\end{itemize}
\begin{align*}
	f = \left(
		\begin{array}{cccc|cccc|ccccc|cccc}
			1&2&\cdots&p&p+1&p+2&\cdots&2p&2p+1&2p+2&\cdots&3p-1&3p&3p+1&\cdots&4p\\
			4p&4p-1&\cdots&3p+1&p+1&3p&\cdots&2p+2&2p&2p-1&\cdots&p+2&p&p-1&\cdots&1
		\end{array}
	\right)\\
	g = \left(
		\begin{array}{cccc|cccc|ccccc|cccc}
			1&2&\cdots&p&p+1&p+2&\cdots&2p&2p+1&2p+2&\cdots&3p-1&3p&3p+1&\cdots&4p\\
			4p-1&4p-3&\cdots&2p+1&0&2p-2&\cdots&2&1&3&\cdots&2p-3&2p&2p+2&\cdots&???
		\end{array}
	\right) 
\end{align*}

