\part{Exercice 2}

{
	\renewcommand{\i}{\ensuremath{\vec{\imath}}}
	\renewcommand{\j}{\ensuremath{\vec{\jmath}}}

	On a $\vec{OM} = \alpha \i + \beta \j$ donc $\Mat_\mathcal{B}\left( \vec{OM} \right) = \begin{pmatrix}
		\alpha\\
		\beta
	\end{pmatrix}$ et
	$\vec{O'M} = \alpha' \vec{u} + \beta' \vec{v}$  donc $\Mat_\mathcal{C}\left( \vec{O'M} \right) =\begin{pmatrix}
		\alpha'\\
		\beta'
	\end{pmatrix}$.

	On a $\vec{O'M} = \vec{O'O} + \vec{OM}$ et $\Mat_\mathcal{C}\left( \vec{O'O} \right) = -\Mat_\mathcal{C}\left( \vec{OO'} \right)$.

	$\vec{OO'} = a \i + b \j$ donc $\Mat_\mathcal{B}\left( \vec{O O'} \right) = \begin{pmatrix}
		a\\b
	\end{pmatrix}$.

	On a $P = P_{\mathcal{B} \to \mathcal{C}} = \begin{pmatrix}
		x&x'\\
		y&y'
	\end{pmatrix}$ et donc $P^{-1} = \frac{1}{xy' - yx'} \begin{pmatrix}
		y'&-x'\\
		-y&x
	\end{pmatrix}$.

	Or, \[
		\forall \vec{w} \in \vec{E},\,\Mat_{\mathcal{C}}\left( \vec{w} \right) = P^{-1} \Mat_{\mathcal{B}}\left( \vec{w} \right)
	.\]

	Donc,
	\begin{align*}
		\begin{pmatrix}
			\alpha'\\
			\beta'
		\end{pmatrix} &= -P^{-1} \begin{pmatrix}
			a\\b
		\end{pmatrix} + P^{-1} \begin{pmatrix}
			\alpha\\\beta
		\end{pmatrix}\\
		&= P^{-1} \begin{pmatrix}
			\alpha - a\\
			\beta - b
		\end{pmatrix} \\
		&= \frac{1}{xy'-yx'} \begin{pmatrix}
			y'(\alpha - x) - x'(\beta - b)\\
			-y(\alpha - a)  + x(\beta - b)
		\end{pmatrix}. \\
	\end{align*}
}

