\part{Sommes doubles}

\begin{exm}
	\[
		S = \sum_{i=1}^n \sum_{j=1}^i a_{i,j}
	\]
	\begin{align*}
		S &= \sum_{j=1}^1 a_{1,j} + \sum_{j=1}^2 a_{2,j} + \sum_{j=3}^3 a_{3,j} + \cdots + \sum_{j=1}^n a_{n,j}\\
		&= a_{11} \\
		&+ a_{21} + a_{22} \\
		&+ a_{31} + a_{32} + a_{33} \\
		&~~\vdots\\
		&+ a_{n,1} + \cdots + a_{n,n}
	\end{align*}
\end{exm}

\begin{exm}
	\begin{align*}
		\sum_{i=1}^n \sum_{j=1}^i&= \sum_{i=1}^n (2^i - 1) \\
		&= \sum_{i=1}^n 2^i - n \\
		&= 2\times \frac{1 - 2^n}{1 - 2} - n \\
		&= 2(2^n - 1) - n \\
	\end{align*}~\\
\end{exm}

\begin{exm}
	Soit $n \in \N^*$.
	\[
		\Bigg.
			S = \sum_{j=1}^i \sum_{i=1}^n {i\choose j}
		\Bigg]\text{\large Aucun sens !}
	\]
\end{exm}

\begin{exm}
	Soit $n \in \N^*$. \[
		S = \sum_{i=1}^n \sum_{j=i}^n {i\choose j} 
	\] On pose \[
		a_{j,i} = {i\choose j}.
	\] Alors,
	\[
		\begin{array}{cccccccc|c|}
			\cline{9-9}
			S &=& a_{11} &+& a_{12} &+& \cdots &+& a_{1n}\\
				&&&+&a_{22} &+& \cdots &+& a_{2n}\\
				&&&&&&\ddots&\vdots&\vdots\\
				&&&&&&&+&a_{nn}\\\cline{9-9}
		\end{array}
	\]
	\[
		\begin{array}{rlccrl}
			\sum_{j=1}^{i} a_{j,i} &= \sum_{j=1}^i {i \choose j} &&&
			\boxed{\cdot} &= \sum_{j=1}^n a_{j,n} = \sum_{j=1}^n {n\choose j} \\
			&= 2^{i}-1&&&&=2^{n} - 1 \\
		\end{array}
	\]

	Donc, \[
		\sum_{i=1}^n\sum_{j=1}^{i} {i\choose j} = 2(2^{n}-1)-n.
	\]
\end{exm}
