\part{Exercice 1}

On a $A = \begin{pmatrix}
	a&1\\
	0&a
\end{pmatrix}$ 

\begin{enumerate}
	\item
		On a $A^2 = \begin{pmatrix}
			a^2&2a\\
			0&a^2
		\end{pmatrix}$, $A^3 = \begin{pmatrix}
			a^3&3a^2\\
			0&a^3
		\end{pmatrix}$, $A^4 = \begin{pmatrix}
			a^4&4a^3\\
			0&a^4
		\end{pmatrix}$.
	\item On pose $\forall n \in \N, \mathcal{P}(n): ``A^n = \begin{pmatrix}
			a^n&na^{n-1}\\
			0&a^n
		\end{pmatrix}"$ \\

		\begin{itemize}
			\item Pour $n = 0$, $\begin{pmatrix}
					a^0&0\\
					0&a^0
				\end{pmatrix} = \begin{pmatrix}
					1&0\\
					0&1
				\end{pmatrix} = I_2 = A^0$\\
				Donc $\mathcal{P}(0)$ est vraie
			\item Soit $n \in \N$, on suppose $\mathcal{P}(n)$ vraie. On a donc $A^n = \begin{pmatrix}
				a^n&na^{n-1}\\
				0&a^n
			\end{pmatrix}$. Montrons $\mathcal{P}(n+1)$.\\
			\begin{align*}
				A^{n+1} = A^n \times A &= \begin{pmatrix}
					a^n&na^{n-1}\\
					0&a^n
				\end{pmatrix} \times \begin{pmatrix}
					a&1\\
					0&a
				\end{pmatrix}\\
				&= \begin{pmatrix}
					a^{n+1}&(n+1)a^n\\
					0&a^{n+1}
				\end{pmatrix}  \\
			\end{align*}
		\end{itemize}
		Donc, $\forall n \in \N, A^n = \begin{pmatrix}
			a^n&na^{n-1}\\
			0&a^n
		\end{pmatrix}$
\end{enumerate}
