\part{Exercice 1}

\begin{enumerate}
	\item
		\begin{align*}
			\forall n \in \N^*, \sum_{k=1}^n \frac{1}{k(k+1)} &= \sum_{k=1}^n \left( \frac{1}{k} - \frac{1}{k+1} \right) \\
			&= 1 - \frac{1}{n+1}\tendsto{n\to +\infty} 1. \\
		\end{align*}
	\item $e : \sum_{n=0}^{+\infty} \frac{1}{n!}$ donc
		\begin{align*}
			\forall n \in \N, \sum_{k=0}^n \frac{k^2+1}{k!} &= \sum_{k=0}^n \frac{1}{k!} + \sum_{k=1}^n \frac{k-1+1}{(k-1)!} \\
			&= \sum_{k=0}^n \frac{1}{k!} + \sum_{k=1}^n \frac{1}{(k-1)!} + \sum_{k=2}^n \frac{1}{(k-2)!} \\
			&\tendsto{n\to +\infty} e + e + e = 3e.
		\end{align*}
	\item Soit $n \in \N$ avec $n \ge 2$.
		\begin{align*}
			\sum_{k=2}^n \ln\left( 1-\frac{1}{k^2} \right) &= \sum_{k=2}^n \ln\left( \frac{(k-1)(k+1)}{k^2} \right) \\
			&= \sum_{k=2}^n \big(\ln(k-1)-\ln(k)\big) + \sum_{k=2}^n \big(\ln(k+1)-\ln(k)\big) \\
			&= -\ln(n) + \ln(n+1) - \ln(2) \\
			&= \ln\left( 1+\frac{1}{n} \right) - \ln(2) \\
			&\tendsto{n\to +\infty} -\ln(2).
		\end{align*}
\end{enumerate}
