\part{Exercice 2}

\begin{align*}
	\forall n \in \N,\, \frac{1}{1+n+n^2} &= \frac{n+1-n}{1+n(n+1)} \\
\end{align*}

On pose \[
	\forall n \in \N,\, u_n = \Arctan n
\] et alors \[
	\forall n \in \N,\, \frac{1}{1+n+n^2} = \frac{\tan u_{n+1} - \tan u_n}{1+ \tan(u_{n+1})\tan(u_n)} = \tan(u_{n+1}-u_n).
\] En effet, \[
	\begin{cases}
		0 < u_{n+1} < \frac{\pi}{2}\\
		-\frac{\pi}{2} < -u_n \le 0
	\end{cases}
\] donc \[
	-\frac{\pi}{2} < u_{n+1} - u_n < \frac{\pi}{2}
\] et donc $u_{n+1} - u_n \not\equiv \frac{\pi}{2} \mod \pi$ et $\Arctan\big(\tan(u_{n+1}-u_n)\big) = u_{n+1}-u_n$.

\begin{align*}
	\forall n \in \N, \sum_{k=0}^n \Arctan\left( \frac{1}{1+k+k^2} \right) &= \sum_{k=0}^n (u_{k+1}- u_k) \\
	&= u_{n+1} - u_n \\
	&\tendsto{n\to +\infty} \frac{\pi}{2}
\end{align*}

On a donc \[
	\frac{\pi}{2} = \sum_{n=0}^{+\infty} \Arctan \left( \frac{1}{1+n+n^2} \right)
\]

