\part{Exercice 3}

\begin{enumerate}
	\item \[
			\forall n \in \N, 0 \le u_n \le \frac{n\,n!}{(n+3)!} = \frac{n}{(n+1)(n+2)(n+3)} \sim \frac{1}{n^2}
		\] $\Sigma u_n$ converge.
	\item \[
			\forall n \ge 2, 0 \le \frac{\ln n}{n^3} = \po\left( \frac{n}{n^3} \right) = \po\left( \frac{1}{n^2} \right)
		\] $\sum \frac{1}{n^2}$ converge donc $\sum \frac{\ln n}{n^3}$ converge.
	\item $\forall \alpha, \ln n = \po(n^\alpha)$. Avec $\alpha = \frac{1}{2}$, on a \[
			0 \le \frac{\ln n}{n^2} = \po\left( \frac{1}{n^{\frac{3}{2}}} \right)
		\] donc $\sum \frac{\ln n}{n^2}$ converge.
	\item $\forall n \ge 3, \frac{\ln n}{n} \ge \frac{1}{n} \ge 0$ donc $\sum \frac{\ln n}{n}$ diverge.
	\item $\left| \frac{(-1)^n}{n^2} \right| = \frac{1}{n^2}$ donc $\sum \frac{(-1)^n}{n^2}$ converge absolument donc $\sum \frac{(-1)^n}{n^2}$ converge.
\end{enumerate}

