\part{Exercice 10}

\begin{enumerate}
	\item Oups, j'ai supprimé cette partie.
	\item
		Si $\alpha > 0$,
		\begin{align*}
			u_n &= \frac{(-1)^n}{n^{\alpha} (-1)^n} = \frac{(-1)^n}{n^\alpha} \times \frac{1}{1 + \frac{(-1)^n}{n^\alpha}}\\
			&= \frac{(-1)^n}{n^\alpha} \left( 1 - \frac{(-1)^n}{n^\alpha} + \po\left( \frac{1}{n^\alpha} \right) \right) \\
			&= \underbrace{\frac{(-1)^n}{n^\alpha}}_{\substack{\text{série alternée}\\\text{convergente}}} - \underbrace{\frac{1}{n^{2\alpha}} + \po\left( \frac{1}{n^{2\alpha}} \right)}_{\sim \frac{1}{n^{2\alpha}} > 0} \\
		\end{align*}

		$\sum \frac{1}{n^{2\alpha}}$ converge si et seulement si $\alpha > \frac{1}{2}$.

		Si $\alpha < 0$, \[
			u_n = \frac{1}{1+(-1)^n n^\alpha} \tendsto{n\to +\infty} 1 \neq 0
		\] donc $u_n$ diverge.
	\item~\\
		\begin{figure}[H]
			\centering
			\begin{asy}
				size(3cm);
				draw(unitcircle);
				draw(expi(0)--expi(pi/3)--expi(2pi/3)--expi(pi)--expi(4pi/3)--expi(5pi/3)--cycle);
				label("$0$", expi(0), align=E);
				label("$\sfrac{\pi}{3}$", expi(pi/3), align=NE);
				label("$\sfrac{2\pi}{3}$", expi(2pi/3), align=NW);
				label("$\pi$", expi(pi), align=W);
				label("$\sfrac{4\pi}{3}$", expi(4pi/3), align=SW);
				label("$\sfrac{5\pi}{3}$", expi(5pi/3), align=SE);
			\end{asy}
		\end{figure}

		\begin{align*}
			S_{6n} &= \sum_{k=1}^{6n} \ln\left( 1+ \frac{\sin(k\pi / 3)}{k} \right) \\
			&= \sum_{a=0}^{n-1}\sum_{k=1}^6 \ln\left( 1 + \frac{\sin\left( \frac{(6a + k) \pi}{3} \right)}{6a + k} \right) \\
			&= \sum_{a=0}^{n-1} \left(
				\ln\left( 1+ \frac{\sqrt{3}}{2(6a + 1)} \right)
				+\ln\left( 1+ \frac{\sqrt{3}}{2(6a + 2)} \right)
				+\ln\left( 1- \frac{\sqrt{3}}{2(6a + 4)} \right)
				+\ln\left( 1- \frac{\sqrt{3}}{2(6a + 5)} \right)
			\right) \\
			&= \sum_{a=0}^{n-1} \Bigg(\ln\left( 1- \frac{\sqrt{3}}{2(6a+4)} + \frac{\sqrt{3}}{2(6a+1)} - \frac{3}{4(6a+1)(6a+4)} \right)\Bigg.\\
			&\phantom{=}\,+ \Bigg(\ln\left( 1-\frac{\sqrt{3}}{2(6a + 5)} + \frac{\sqrt{3}}{2(6a + 2)} - \frac{3}{4(6a+2)(6a+5)} \right) \Bigg) \\
			&= \sum_{a=0}^{n-1} \ln\left( 1 + \frac{6\sqrt{3} - 3}{4(6a + 1)(6a+4)} \right) 
			+ \sum_{a=0}^{n-1} \ln\left( 1 + \frac{6\sqrt{3} - 3}{4(6a+2)(6a+5)} \right)\\
		\end{align*}
\end{enumerate}

 \[
	\ln\left( 1 + \frac{6\sqrt{3} - 3}{4(6a + 1)(6a + 4)} \right) \simi_{a\to +\infty} \frac{6\sqrt{3} - 3}{4 \times  36a^2} > 0.
\]
$\sum \frac{6\sqrt{3} - 3}{4 \times 36a^2}$ converge donc $\sum \ln \left( 1 + \frac{6 \sqrt{3} - 3}{4(6a + 4)(6a+1)} \right)$ converge.

Donc $(S_{6n})$ converge.\\
$S_{6n+1} = S_{6n} + \underbrace{u_{6n+1}}_{\to 0} \longrightarrow \lim S_{6n}$ \\
$S_{6n+2},\ldots,S_{6n+5} \longrightarrow \lim S_{6n}$

donc $(S_n)$ converge et donc $\Sigma u_n$ converge.


