\part{Exercice 2}

\begin{enumerate}
	\item
		\begin{align*}
			X^4 + 1 &= (X^2+1)^2 - 2X^2\\
			&= \left(X^2 + 1 - \sqrt{2}X\right)\left(X^2 +1-\sqrt{2}X\right) \\
		\end{align*}
	\item
		\begin{align*}
			X^5 - 1 &= (X-1)\left( X^4 + X^3 + X^2 + X + 1 \right) \\
		\end{align*}
	\item~\\
		\begin{center}
			$\begin{array}
				{c|c c c c c}
				&1&-2&3&-2&2\\ \hline
				i&1&-2+i&2-2i&2i&0\\ \hline
				-i&1&-2&-2&0&0
			\end{array}$
		\end{center}
		\begin{align*}
			(X^2 - X + 1)^2 + 1 &= (X^2+1)(X^2-2x-2)\\
		\end{align*}
\end{enumerate}

