\part{Exercice 2}

\begin{enumerate}
	\item
		\begin{itemize}
			\item[$``i \implies ii"$]
				\begin{align*}
					\forall a,b \in G, (ab)^2 &= abab\\
					&= aabb \\
					&= a^2b^2 \\
				\end{align*}
			\item[$``ii\implies i"$ ]
				\begin{align*}
					\forall (a,b) \in G^2, abab &= a^2b^2\\
					&\text{donc } bab=a b^2 \\
					&\text{donc } ba = ab \\
				\end{align*}
			\item[$`ì \implies iii"$]
				\begin{align*}
					\forall a,b \in G, (a,b)^{-1} = b^{-1}a^{-1} = a^{-1}b^{-1}
				\end{align*}
			\item[$``iii \implies i"$]
				\begin{align*}
					\forall a,b \in G, ab = \left( b^{-1}a^{-1} \right) ^{-1} = \left( b^{-1} \right) ^{-1} = ba
				\end{align*}
		\end{itemize}
	\item
		Soit $a,b \in G$ \\
		\begin{itemize}
			\item $(a,b)^2 = e$
			\item $a^2 b^2 = e \cdot e = e$
		\end{itemize}
		Donc, $(a,b)^2 = a^2b^2$ donc $G$ est abélien
\end{enumerate}

