\part{Exercice 10}

\[
	\Z[i] = \{a+ib  \mid (a,b) \in \Z^2\} 
\]

\begin{itemize}
	\item $\Z[i] \subset  \C$ 
	\item Soient $u,v \in \Z[i]$. On pose $u = a + ib$ et $v = c+id$ avec $(a,b,c,d) \in \Z^4$.\\
		\begin{align*}
			u+v &= \underbrace{(a+c)}_{\in \Z} + i\underbrace{(b+d)}_{\in \Z} \in \Z[i]\\
			uv &= \underbrace{(ac-bd)}_{\in \Z} + i\underbrace{(ad+bc)}_{\in \Z} \in \Z[i]\\
		\end{align*}

		\begin{align*}
			- u &= -a - ib  \in \Z[i]\\
			0 &= 0 + i \times 0 \in \Z[i]
			1 &= 1 + i \times 0 \in \Z[i]
		\end{align*}
	\item Soit $u \in \Z[i]^\times$. On sait qu'il existe $v \in \Z[i]$ tel que $uv = 1$.\\
		Donc, $\left| u \right|^2\left| v \right| ^2 = \left| uv \right| ^2 = 1^2=1$ \\
		Comme $u \in \Z[i]$, $\left| u \right| ^2 = \Re(u)^2 + \Im(u)^2 \in \N$ \\
		De même, $\left| v \right| ^2 \in \N$ \\
		Donc, $\left| u \right| ^2 = 1$.

		% schema 1

		On pose $u = a+ib, (a,b) \in \Z^2$. On a $a^2 + b^2 = 1$\\
		donc $\begin{cases}
			0 \le a^2 \le 1\\
			0 \le b^2 \le 1\\
		\end{cases}$ \\
		Donc, $\begin{cases}
			a^2 \in \{0,1\} \\
			b^2 \in \{0,1\}\\
			a^2+b^2 = 1
		\end{cases}$ \\
		Donc, $u \in \{\pm i, \pm 1\}$ \\
	\item
		\begin{align*}
			1^{-1} = 1 \in \Z[i]\\
			(-1)^{-1} = -1 \in \Z[i]\\
			i^{-1} = -i \in \Z[i]\\
			(-i)^{-1} = i \in \Z[i]\\
		\end{align*}
	\item[\sc Autre méthode] $u \in \Z[i]\setminus \{0\}$. $u = a+ib$ avec $a,b \in \Z$.\\
		\begin{align*}
			\frac{1}{u} \in \Z[i] &\iff \frac{1}{a+ib}\in \Z[i]\\
														&\iff \frac{a-ib}{a^2-b^2} \in \Z[i]\\
														&\iff \begin{cases}
															\frac{a}{a^2+b^2} \in \Z\\
															\frac{-b}{a^2+b^2} \in \Z
														\end{cases}
														&\iff \begin{cases}
															a^2+b^2 \mid a\\
															a^2+b^2 \mid b\\
														\end{cases}\\
														&\implies \begin{cases}
															a^2+b^2 \le \left| a \right|\\
															a^2+b^2 \le \left| b \right|\\
														\end{cases}
														&\implies \begin{cases}
															a \in \{0,1,-1\}\\
															b \in \{0,1,-1\}\\
															a^2 + b^2 = 1
														\end{cases}
		\end{align*}
\end{itemize}
