\part{Exercice 27}
$n < p$
 \[
	 (p-1)(p-2)\ldots(p-n) = \frac{(p-1)!}{(p-n-1)!}
\] 
Donc,
\begin{align*}
	\frac{(p-1)(p-2)\ldots(p-n)}{n!} &= \frac{(p-1)!}{n!(n-p-1)!}\\
	&= \begin{pmatrix} p-1\\n \end{pmatrix}\\
\end{align*}

\[
	(p-1)(p-2)\ldots(p-n)\equiv(-1)^n n! ~[p]
\] 
$n! = 1 \times  2 \times \ldots \times n$ est premier avec $p$ car $\forall k \in \left\llbracket 1,n \right\rrbracket, k \wedge p = 1$.\\
Donc, $n!$ est inversible modulo $p$. Donc, \[
	\begin{pmatrix} p-1\\n \end{pmatrix} \equiv (-1)^n ~[p]
\]
