\part{Exercice 2}

On pose $\begin{cases}
	M: x \mapsto \max(f(x),g(x))\\
	m: x \mapsto \min(f(x),g(x))\\
\end{cases}$ \\
On remarque que \[
	\forall x \in \R,
	\begin{cases}
		M(x) + m(x) = f(x) + g(x)\\
		M(x) - m(x) = \left| f(x) - g(x) \right| 
	\end{cases}
\]

Donc \[
	\forall x \in \R, M(x) = \frac{1}{2}\left( f(x) + g(x) + \left| f(x) - g(x) \right| \right)
\] et \[
	\bigg(
	\forall x \in \R, m(x) = \frac{1}{2}\left( f(x) + g(x) - \left| f(x) - g(x) \right| \right)
	\bigg)
\]
On a bien $M$ continue
