\part{Exercice 6}

\begin{enumerate}
	\item On pose $g : (x,y) \mapsto f(y, x)$.

		\begin{align*}
			\frac{\partial g}{\partial x}(x,y) &= \frac{\partial f}{\partial x}(y,x)\;\frac{\partial y}{\partial x}(x,y) + \frac{\partial f}{\partial y}(y,x)\;\frac{\partial x}{\partial x}(x,y)\\
			&= \frac{\partial f}{\partial y}(y,x) \\
		\end{align*}

		\begin{align*}
			\frac{\partial g}{\partial y}(x,y) &= \frac{\partial f}{\partial x}(y,x)\; \frac{\partial x}{\partial x}(x,y) + \frac{\partial f}{\partial y}(y,x)\; \frac{\partial y}{\partial x}(x,y) \\
			&= \frac{\partial f}{\partial x}(y,x) \\
		\end{align*}
	\item On pose $h: (x,y) \mapsto f\big(y, f(x,x)\big)$ et $k : x \mapsto f(x,x)$

		\begin{align*}
			\frac{\partial h}{\partial x}(x,y) &= \frac{\partial f}{\partial x}\big(y, f(x,x)\big)\;\frac{\partial y}{\partial x}(x,y) + \frac{\partial f}{\partial y}\big(y, f(x,x)\big)k'(x)\\
			&= \frac{\partial f}{\partial y}\big(y, f(x,x)\big)  \left( \frac{\partial f}{\partial x}(x,x) + \frac{\partial f}{\partial y}(x,x) \right)\\
		\end{align*}

		En effet, on a $\gamma: x \mapsto (x,x)$ et $\gamma'(x) = (1,1)$.

		Donc $f \circ \gamma : x \mapsto f(x,x) = k(x)$.
		\begin{align*}
			k'(x) &= \left<\nabla f(x,x)  \mid \gamma'(x) \right> \\
			&= \frac{\partial f}{\partial x}(x,x) + \frac{\partial f}{\partial y}(x,x).
		\end{align*}

		\begin{align*}
			\frac{\partial h}{\partial y}(x,y) &= \frac{\partial f}{\partial x}\big(y, f(x,x)\big) \frac{\partial f}{\partial y}(x,y) + \frac{\partial f}{\partial y}\big(y, f(x,x)\big) \times 0\\
			&= \frac{\partial f}{\partial x}\big(y, f(x,x)\big). \\
		\end{align*}
\end{enumerate}
