\part{Exercice 7}

Soit $u = (a,b) \in \R^2$.

\[
	\forall t \neq 0, \Delta f(t) = \frac{f\big((0,0) - tu\big) - f(0,0)}{t} = \frac{1}{t} f(ta, tb).
\]

\begin{itemize}
	\item[\underline{\sc Cas 1}] $a \neq 0$. Alors, \[
			\forall t \neq 0, \Delta f(t) = \frac{1}{t}t^2b^2\ln\big(|ta|\big) = tb^2\ln\big(|ta|)\big) \tendsto{t\to 0} 0.
		\]
	\item[\underline{\sc Cas 2}] $a = 0$. Alors, \[
			\Delta f(t) = \frac{1}{t} \times 0 = 0 \tendsto{t\to 0} 0.
		\]
\end{itemize}

On trouve que \[
	\forall u \in \R^2, \mathrm{d}f(u)(0,0) = 0.
\]
On pose \[
	\begin{cases}
		x(t) = t\\
		y(t) = \begin{cases}
			0 &\text{ si } t = 0\\
			\sqrt{\frac{1}{\left| \ln\big(|t|\big) \right|}} &\text{ si } t \neq 0
		\end{cases}
	\end{cases}
\] et on a bien \[
	\begin{cases}
		x(t)\tendsto{t\to 0} 0\\
		y(t)\tendsto{t\to 0} 0\\
	\end{cases}
\]

On a \[
	\lim_{t\to 0}f\big(x(t), y(t)\big) = -1 \tendsto{t\to 0} -1 \neq f(0,0)
\]

\centered{***}

On a \[
	\begin{cases}
		\frac{\partial f}{\partial x}(0,0) = \mathrm{d}f(1,0)(0,0) = 0,\\[3mm]
		\frac{\partial f}{\partial y} = \mathrm{d}f(0,1)(0,0) = 0.
	\end{cases}
\] et \[
	\forall (x,y) \in \R^* \times \R,
	\begin{cases}
		\frac{\partial f}{\partial x}(x,y) = \frac{y^2}{|x|} \times \sgn(x) \tendsto{x\to 0} \pm\infty\\[3mm]
		\frac{\partial f}{\partial y}(x,y) = 2y \ln\big(|x|\big).
	\end{cases}
\]
