\part{Exercice 12}

\begin{enumerate}
	\item $\begin{cases}
			\frac{\partial f}{\partial x} = xy^2\\[2mm]
			\frac{\partial f}{\partial y} = x^2 y
		\end{cases}$ 

		Donc $f(x,y) = \frac{x^2y^2}{2} + \lambda$.
	\item $\begin{cases}
			\frac{\partial f}{\partial x} = \frac{x}{\sqrt{x^2+y^2}}\\[2mm]
			\frac{\partial f}{\partial y} = \frac{y}{\sqrt{x^2 + y^2}}
		\end{cases}$ 

		Donc $f(x,y) = \sqrt{x^2 + y^2} + \lambda$.
	\item $\begin{cases}
			\frac{\partial f}{\partial x} = \frac{x}{x^2 + y^2}\\[2mm]
			\frac{\partial f}{\partial y} = -\frac{y}{x^2 + y^2}
		\end{cases}$ 

		D'après $(E_1)$,  $f(x,y) = \frac{1}{2} \ln\big(x^2 + y^2\big) + g(y)$

		Or, 
		\[
			\frac{\partial f}{\partial y} = \frac{y}{x^2 + y^2} + g'(y) = -\frac{y}{x^2 + y^2}
			\iff g'(y) = \frac{2y}{x^2 + y^2} \text{ dépend de $x$}\kern 2mm \lightning
		\] 
\end{enumerate}

