\part{Motivation}

La série $\sum \frac{(-1)^n}{n}$ est semi-convergente. On a $\sum_{n=1}^{+\infty} \frac{(-1)^n}{n} = -\ln 2$, d'où, \[
	-1 + \frac{1}{2} - \frac{1}{3} + \frac{1}{4} - \frac{1}{5} + \frac{1}{6} + \cdots = -\ln 2
.\]

On change l'ordre :
\begin{align*}
	&\overbrace{-1 + \frac{1}{2} + \frac{1}{4}}^{-\frac{1}{2} +\frac{1}{4}} - \overbrace{\frac{1}{3} + \frac{1}{6} + \frac{1}{8}}^{-\frac{1}{6} + \frac{1}{8}} - \overbrace{\frac{1}{5} + \frac{1}{10} + \frac{1}{12}}^{-\frac{1}{10}  + \frac{1}{12}} + \cdots\\
	&= \frac{1}{2} \left( -1 + \frac{1}{2} - \frac{1}{3} + \frac{1}{4} - \frac{1}{5} + \frac{1}{6} + \cdots \right) \\
	&= \frac{-\ln 2}{2} \\
\end{align*}

\begin{thm}[réarrangement de Riemann]
	Soit $\Sigma u_n$ une série semi-convergente réelle. \[
		\forall \ell \in \R,\,\exists \sigma : \N \xrightarrow{\text{bij}} \N,\,
		\sum_{n=1}^{+\infty} u_{\sigma(n)} = \ell
	.\]
\end{thm}

