\part{Exercice 4}

Soit \[
	g_M: x\mapsto f(x) - f(a) - \frac{x-a}{2}\big(f'(x) + f'(a)\big) - (x-a)^3M
\] 
$g_M$ est continue sur $[a,b]$ et dérivable sur $]a,b[$ \\
$g_M(a) = 0$ \\
$g_M(b) = f(b) - f(a) - \frac{b-a}{2}\big(f'(b) - f'(a)\big) - (b-a)^3M$ \\
On pose $M = \frac{1}{(b-a)^3}\left( f(b) - f(a) - \frac{b-a}{2} \big(f'(b) + f'(a)\big) \right) $ \\
Ainsi, $g_M (b) = 0$\\
D'après le théorème de Rolle, il existe $\gamma \in ]a,b[$ tel que $g'_M(\gamma) = 0$ \\
D'où, 
\begin{align*}
	0 
	&= f'(\gamma) - \frac{1}{2}\big(f'(\gamma) + f'(a)\big) - \frac{\gamma - a}{2}f''(\gamma) - 3 (\gamma-a)^2M\\
	&= \frac{1}{2}\big(f'(\gamma)  -f'(a)\big) - \frac{\gamma-a}{2}f''(\gamma) - 3(\gamma - a) ^2M \\
\end{align*}

Or, \[
	g'_M(a) = 0
\]
\begin{itemize}
	\item $g'_M$ est continue sur $[a,\gamma]$
	\item $g'_M$ est dérivable sur $]a,\gamma[$ 
	\item $g'_M(a) = g'_M(\gamma)$
\end{itemize}
Donc, il existe $c \in ]a,\gamma[ \subset ]a,b[$ tel que \[
	g''_M(c) = 0
\] d'où $M = -\frac{1}{12} f^{(3)}(c)$ \\
On en déduit \[
	f(b) = f(a) + \frac{b-a}{2}\big(f'(b) + f'(a) \big) - \frac{(b-a)^3}{12} f^{(3)}(c)
\]


