\part{Exercice 2}

%\begin{align*}
	%\alpha'u + \beta' v = \alpha i + \beta j \iff& \alpha' xi + \alpha'yi + \beta' x'i + \beta' y'j = \alpha i + \beta j  \\
	%\iff& \begin{cases}
		%\alpha' x + \beta' x' = \alpha\\
		%\alpha' y + \beta' y' = \beta
	%\end{cases}\\
	%\iff& \begin{pmatrix}
		%x&x'\\
		%y&y'
	%\end{pmatrix} \begin{pmatrix}
		%\alpha'\\
		%\beta'
	%\end{pmatrix} = \begin{pmatrix}
		%\alpha\\
		%\beta
	%\end{pmatrix}\\
	%\iff& \begin{cases}
		%\begin{vmatrix}
			%x&x'\\
			%y&y'
		%\end{vmatrix} \neq 0\\
		%\begin{pmatrix}
			%\alpha'\\
			%\beta'
		%\end{pmatrix} = 
		%\begin{pmatrix}
			%x&x'\\
			%y&y'
		%\end{pmatrix}^{-1} \begin{pmatrix}
			%\alpha\\
			%\beta
		%\end{pmatrix}
	%\end{cases}\\
	%\iff& \begin{cases}
		%xy' - yx' \neq 0\\
		%\begin{pmatrix}
			%\alpha'\\
			%\beta'
		%\end{pmatrix} = \frac{1}{xy'-y'x} \begin{pmatrix}
			%y'&-x'\\
			%-y&x
		%\end{pmatrix} \begin{pmatrix}
			%\alpha\\
			%\beta
		%\end{pmatrix}
	%\end{cases}\\
	%\implies& \begin{cases}
		%\alpha' = \frac{y' \alpha - x' \beta}{xy'-y'x}\\
		%\beta' = \frac{-y \alpha - x \beta}{xy'-y'x}\\
	%\end{cases}
%\end{align*}

On pose la matrice du repère $(O, u, v)$ :  \[
	M = \begin{pmatrix}
		x&x'&a\\
		y&y'&b\\
		0&0&1
	\end{pmatrix} 
.\]

On a donc \[
	\begin{pmatrix}
		x&x'&a\\
		y&y'&b\\
		0&0&1
	\end{pmatrix} \begin{pmatrix}
		\alpha'\\
		\beta'\\
		0\\
	\end{pmatrix} = \begin{pmatrix}
		\alpha\\
		\beta\\
		0
	\end{pmatrix}
.\]

On cherche donc $\begin{pmatrix}
	x&x'&a\\
	y&y'&b\\
	0&0&1
\end{pmatrix}^{-1}$.

\begin{align*}
	\left(
		\begin{array}{ccc|ccc}
			x&x'&a&1&0&0\\
			y&y'&b&0&1&0\\
			0&0&1&0&0&1
		\end{array}
	\right)
	\begin{array}{c}
		\sim\\
		\substack{L_1 \leftarrow L_1 - aL_3\\L_2\leftarrow L_2-bL_3}
	\end{array}&
	\left(
		\begin{array}{ccc|ccc}
			x&x'&0&1&0&-a\\
			y&y'&0&0&1&-b\\
			0&0&1&0&0&1
		\end{array}
	\right)
\end{align*}

On a \[
	\begin{pmatrix}
		x&x'\\
		y&y'
	\end{pmatrix}^{-1} = \frac{1}{xy'-yx'} \begin{pmatrix}
		y'&-x'\\
		-y&x
	\end{pmatrix}
.\] D'où \[
	M^{-1} = \begin{pmatrix}
		\frac{y'}{xy' - yx'}&-\frac{x'}{xy' - yx'}&-a\\
		-\frac{y}{xy'-yx'}&\frac{x}{xy'-yx'}&-b\\
		0&0&1
	\end{pmatrix} 
.\] On en déduit que \[
	\begin{cases}
		\alpha' = \frac{\alpha y' - \beta x'}{xy' - yx'} - a\\[2mm]
		\beta' = \frac{\alpha x - \beta y}{xy' - yx'} - b\\
	\end{cases}
.\]
