\part{Exercice 2}

Soit $(\Omega, P)$ un espace probabilisé modélisant la situation.

\begin{enumerate}
	\item On a $X(\Omega) = \left\llbracket 2,n-1 \right\rrbracket$.
		\[
			\forall k \in \left\llbracket 2,n-1 \right\rrbracket,\, P(X = k) = \frac{(k-1)(n-k)}{{n\choose 3}}
		.\]

		\underline{Vérification} :
		\begin{align*}
			\sum_{k=0}^n P(X = k) &= \frac{3!\:(n-3)!}{n!} \sum_{k=2}^{n-1} \big(-k^2 + (n+1)k - n\big) \\
			&= \frac{6}{n(n-1)(n-2)} \left( - \frac{(n-1)\,n\,(2n-1)}{6} + 1 + (n+1) \frac{(n-2)(n+1)}{2} - n\,(n-2) \right) \\
			&= \frac{6}{n(n-1)(n-2)} \times \frac{-n(n-1)(2n-1) + 6 + 3(n+1)^2 + (n-2) - 6n(n-2)}{6} \\
			&= \frac{1}{n^3 -3n^2 + 2n} \times \left( n^3 - 3n^2 + 2n \right)  \\
			&= 1. \\
		\end{align*}
	\item
		\begin{align*}
			E(X) = \sum_{k=2}^{n-1} k \frac{(k-1)(n-k)}{{n\choose 3}} = \cdots\cdots\cdots
		\end{align*}
\end{enumerate}
