\part{Exercice 7}

\[
	X = \sum_{i=1}^{Np} X_i \quad \text{ d'où } \quad E(X) = \sum_{i=1}^{Np} E(X_i)
.\]

Or, $X_i\textstyle \sim \mathcal{B}\left( \frac{{N-1\choose n-1}}{{N\choose n}} \right)$.

On en déduit que
\begin{align*}
	E(X) &= \sum_{i=1}^{Np} \frac{{N-1\choose n-1}}{{N \choose n}}\\
	&= \frac{n!\:\cancel{(N-n)!}\:(N-1)!\:Np}{N!\:(n-1)!\:\cancel{(N-n)!}} \\
	&= \frac{n}{N}Np \\
	&= np. \\
\end{align*}

\[
	V(X) = \sum_{i=1}^{Np} V(x_i) + 2\sum_{1\le i<j}\Cov(X_i, X_j)
\] où \[
	\Cov(X_i, X_j) = E(X_iX_j) - E(X_i)E(X_j)
.\]


\begin{enumerate}
	\item $X_i \sim \mathcal{B}\left( \frac{{N-1\choose n-1}}{{N\choose n}} \right)$.
		\[
			E(X_i) = \frac{n!\:(N-n)!}{N!} \times \frac{(N-1)!}{(n-1)!\:(N-n)!} = \frac{n}{N}
		.\]
		\[
			V(X_i) = \frac{n}{N}\left( 1-\frac{n}{N} \right) = \frac{n(N-n)}{N^2}
		.\]
	\item $\Cov(X_i, X_j) = E(X_iX_j)-E(X_i)E(X_j)$. Or, $X_iX_j \sim \mathcal{B}\big(P(X_i = 1, X_j = 1)\big)$ et
		\begin{align*}
			P(X_i = 1, X_j = 1) &= \frac{{N-2\choose n-2}}{{N \choose n}}\\
			&= \frac{(N-2)!}{(n-2)!\:\cancel{(N-n)!}} \times \frac{n!\:(N-n)!}{N!}\\
			&= \frac{n(n-1)}{N(N-1)}. \\
		\end{align*}
	\item On a $X = \sum_{i=1}^{Np}X_i$ et donc \[
			E(X) = \sum_{i=1}^{Np}E(X_i) = \frac{n}{N} \times N p = np
		\] et
		\begin{align*}
			V(X) &= \sum_{i=1}^{Np}V(X_i) + \sum_{1\le i \neq j \le Np} \Cov(X_i, X_j) \\
			&= p \frac{n}{N} (N - n) + \cancel{N}p(Np-1) \frac{n(n-1)}{\cancel{N}(N-1)}. \\
		\end{align*}

		\underline{Loi de $X$} : \[
			P(X = k) = \frac{{Np \choose k}{Nq \choose n-k}}{{N \choose n}}
		.\]
\end{enumerate}
